pulse/examples/steel/arraystructs/AggregateRef.fst
@@ -154,13 +154,59 @@ let un_addr_of_lens #a #b #c #p #q r' r l x y =
   l.put_morphism.f_op (get l x, Ghost.reveal x) (Ghost.reveal y, one p);
   A.change_equal_slprop (r `pts_to` _) (r `pts_to` _)
 
+val refine
+  (#a:Type) (#b:Type) (#p: refined_one_pcm b)
+  (r: ref a p)
+  (re: pcm_refinement p)
+  (x: Ghost.erased b{refinement_f re x})
+: Steel (ref a (refined_pcm re))
+    (r `pts_to` x)
+    (fun r' -> r' `pts_to` Ghost.reveal x)
+    (fun _ -> True)
+    (fun _ r' _ -> r' == ref_refine r re)
 let refine r re x =
   let r' = ref_refine r re in
   A.change_equal_slprop (r `pts_to` x) (r' `pts_to` Ghost.reveal x);
   A.return r'
 
+val unrefine
+  (#opened:Steel.Memory.inames)
+  (#a:Type) (#b:Type) (#p: refined_one_pcm b)
+  (r': ref a p)
+  (re: pcm_refinement p)
+  (r: ref a (refined_pcm re))
+  (x: Ghost.erased b{refinement_f re x})
+: A.SteelGhost unit opened
+    (r `pts_to` Ghost.reveal x)
+    (fun _ -> r' `pts_to` x)
+    (fun _ -> r == ref_refine r' re)
+    (fun _ _ _ -> True)
 let unrefine #inames r' re r x =
   A.change_equal_slprop (r `pts_to` Ghost.reveal x) (r' `pts_to` x)
+
+(*
+val addr_of_union_lens
+  (#a:Type) (#b:Type) (#c:Type) (#p: refined_one_pcm b) (#q: refined_one_pcm c)
+  (r: ref a p) (#re: pcm_refinement p) (l: pcm_lens (refined_pcm re) q)
+  (x: Ghost.erased b{refinement_f re x})
+: Steel (ref a q)
+    (r `pts_to` x)
+    (fun s ->
+      (r `pts_to` put l (one q) x) `star` 
+      (s `pts_to` get l x))
+    (requires fun _ -> True)
+    (ensures fun _ r' _ -> r' == ref_focus r l)
+
+val un_addr_of_union_lens
+  (#a:Type) (#b:Type) (#c:Type) (#p: refined_one_pcm b) (#q: refined_one_pcm c)
+  (r': ref a q) (r: ref a p) (l: pcm_lens p q)
+  (x: Ghost.erased b) (y: Ghost.erased c)
+: Steel unit
+    ((r `pts_to` x) `star` (r' `pts_to` y))
+    (fun s -> r `pts_to` put l y x)
+    (requires fun _ -> r' == ref_focus r l /\ get l x == one q)
+    (ensures fun _ _ _ -> True)
+*)
 
 let ref_read (#p: refined_one_pcm 'b) (#x: Ghost.erased 'b) (r: ref 'a p)
 : Steel 'b
