pulse/examples/steel/arraystructs/FStar.PCM.POD.fst
@@ -1,4 +1,4 @@
-module PCM.POD
+module FStar.PCM.POD
 
 let pod a = option a
 
